Call support

examples/sgx/Interpreter.fst
@@ -2,7 +2,7 @@
 module Interpreter
 
 open SGXState
-open FStar.Array
+open FStar.Buffer
 open FStar.UInt64
 open FStar.List
 open Util
@@ -10,7 +10,8 @@ open Ast
 
 exception Halt
 
-let u64 = UInt64.t
+let word = UInt64.t
+let address = UInt64.t
 
 (*
 val STX.Halt: unit -> STX 'a 
@@ -18,20 +19,22 @@ val STX.Load : unit -> buffer ... -> STX word
 val STX.Store: unit -> buffer ... -> STX unit
 *)
 
-val defensive: (array u64) -> (array u64) ->nat-> nat->nat->nat->nat->nat-> sgxstate
-let defensive regs buf base wbmapstart uheapstart ustackstart ucodestart size = 
+assume val search: (buffer word)->(addr:nat)-> bool
+
+val defensive: (buffer word) -> (buffer word)->(buffer word) ->nat-> nat->nat->nat->nat->nat-> sgxstate
+let defensive regs buf calltable base wbmapstart ucodestart uheapstart ustackstart size = 
   let read' (regname:string) = 
        (* What should regs structure be? *)
        0uL
     in
-  let write' (regname:string) (value:u64) = 
+  let write' (regname:string) (value:word) = 
        ()
     in
   let load' (n:nat) (addr:nat) = 
-       Array.index buf (addr-base) 
+       Buffer.index buf (addr-base)
     in
-  let store' (n:nat) (v:u64) (addr:nat) =
-     if addr > wbmapstart && addr < uheapstart then
+  let store' (n:nat) (v:word) (addr:nat) =
+     if addr > wbmapstart && addr < ucodestart then
 	(* addr is in write-bitmap, get the index
 	   i.e. bitmapindex represents the address whose permission
 	   is being toggled 
@@ -44,24 +47,37 @@ let defensive regs buf base wbmapstart uheapstart ustackstart ucodestart size =
 	*)
 	let currentframestart = cast_to_nat (read' "rbp") in
 	if (bitmapindex < currentframestart) then	
-        	Array.upd buf (addr-base) v
+        	Buffer.upd buf (addr-base) v
 	else
 		raise Halt
     else if addr >uheapstart && addr < ustackstart then
-	(* In Progress: Do necessary checks here.. *)  
+	(* In Progress: Address is in UHeap.. *)  
+	()
+    else if addr >ustackstart && addr < (read' "rbp")  then
+	(* In Progress: Address belongs to older stack frames *)  
+	()
+    else if addr >(read' "rbp") && addr < (read' "rsp")  then
+	(* In Progress: Address belongs to current stack frame. Always ok *)  
 	()
     in
-   Mksgxstate read' write' load' store'
+  let iscallableaddress' (addr:nat) =
+	let iscallable = search calltable addr in
+	if iscallable then
+		()
+	else
+		raise Halt
+    in	
+   Mksgxstate read' write' load' store' iscallableaddress'
 	
 (* Should look into the call table from manifest and fetch the corresponding function
  *)
-let decode insaddr = [Skip]
+let decode instraddr = [Skip]
 
 let get_register_name = function
  | Register r -> r
  | _ -> raise Halt
 
-val eval: sgxstate -> exp -> u64
+val eval: sgxstate -> exp -> word
 let eval (env:sgxstate) = function
  | Register r -> env.read r 
  | Constant n -> n
@@ -82,6 +98,8 @@ let rec step (env:sgxstate) = function
        env.write regname value
   | Call e ->
        let fentry = eval env e in
+	(* Raises Exception if the function is not callable *)	
+       let _ = env.iscallableaddress fentry in
 	(* Convert this to sequence of instructions *)
 	steps env (decode fentry)
   | If (e, truli, falsli) ->
@@ -100,8 +118,14 @@ and steps (env:sgxstate) instr = List.iter (fun elem->step env elem ) instr
 (* Should the following function have a type that uses effects associated with hyperstack ? 
    Is buf supposed to be a hyperstack?
 *)
-val ustar:(array u64)->(array u64)-> nat ->nat->nat->nat->nat->unit->unit
-let ustar regs buf base wbmapstart uheapstart ustackstart ucodestart entry = 
+val ustar:(buffer word)->(buffer word)-> (buffer word)->nat ->nat->nat->nat->nat->unit->unit
+let ustar regs buf calltable base wbmapstart uheapstart ustackstart ucodestart entry = 
   let size = 1000 in
-  let mem = defensive regs buf base wbmapstart uheapstart ustackstart ucodestart size in
+  let mem = defensive regs buf calltable base wbmapstart ucodestart uheapstart ustackstart size in
+  (* For testing *)
   steps mem [(Store(1uL,(Register "rax"),(Register "rcx")))] 
+
+(* Place holder for parsing manifest and getting the start addresses and  
+  calltable
+ *)
+let parse_manifest = ()
